
\documentclass{article}
\usepackage[utf8]{inputenc}
\usepackage[russian]{babel}
\usepackage{amsthm}
\usepackage{amsmath}

\begin{document}


Function:
$$
y
$$
Variable:
$$
x
$$

%1.
Equation:
$$
xydx+(x+1)dy=0
$$

Solution:
$$
y=C(x+1)e^{-x}
$$

%2.
Equation:
$$
x\frac{d}{dx}y-2y=bx^3y^2
$$
Solution:
$$
y = \frac{5x^2}{-bx^5+C}
$$

%2\sqrt{Ay(A^2-y^2} + A\frac{d}{dx}y = 0

%3

Equation:
$$
xydx+(x+1)dy=0
$$
Solution:
$$
y=C(x+1)e^{-x}
$$

%4.
Equation:
$$
x\frac{d}{dx}y-2y=bx^3y^2
$$
Solution:
$$
y = \frac{5x^2}{x^5+C}
$$

%\fbox{\textbf{Задачи и упражнения к п.~1.1:}}
%\vspace{3mm}

%\eqn ${}\quad 2\sqrt{Ay(A^2-y^2)}\,dx+A\,dy=0$.
%\vspace{2mm}

%Equation:
%$$
%2\sqrt{Ay(A^2-y^2} + A\frac{d}{dx}y = 0
%$$
%Solution:
%$$
%y=A[\ch(x+C)]^{-2}
%$$

Equation:
$$
\frac{d}{dx}y=(9x+y-1)^2
$$
Solution:
$$
y=-3 \frac{\sin(C-3x)}{\cos(C-3x)} + 1-9x
$$


\end{document}






